



give prove of this

Here is **the complete proof** for the solution logic of **CF 1374B — Multiply by 2, divide by 6**.

✓ Goal

You are given a number n .

You can do two operations:

1. **Multiply by 2** → $n = n * 2$
2. **Divide by 6** (only if $n \% 6 == 0$) → $n = n / 6$

You need the **minimum steps** to reach **1** from n .

✓ Key Insight

To reach 1, the prime factorization must end up as:

$$1 = 2^0 \cdot 3^0.$$

So n must contain only primes 2 and 3.

If any other prime appears → **impossible (return -1)**.

✓ STEP 1 — Factorize

Let:

- cnt2 = number of times 2 divides n
- cnt3 = number of times 3 divides n

Example:

$$n = 72 = 2^3 * 3^2$$

→ `cnt2 = 3` , `cnt3 = 2`

If after dividing out all 2's and 3's, the leftover is not 1 →
there was some other prime → **impossible**.

✓ STEP 2 — Understanding operations in terms of prime factors

Operation 1: multiply by 2

$$n \leftarrow n \times 2$$

→ increases exponent of 2:

$$2^{cnt2} \cdot 3^{cnt3} \rightarrow 2^{cnt2+1} \cdot 3^{cnt3}$$

Operation 2: divide by 6

$$n \leftarrow \frac{n}{6} = \frac{n}{2 \cdot 3}$$

→ reduces exponent of 2 and 3:

$$2^{cnt2} \cdot 3^{cnt3} \rightarrow 2^{cnt2-1} \cdot 3^{cnt3-1}$$

✓ STEP 3 — What must happen to reach `1`?

We want final:

$$2^0 \cdot 3^0$$

After divisions, both exponents must reach zero.

Every **divide by 6** decreases:

- exponent of 2 → minus 1
- exponent of 3 → minus 1

This is the only operation that reduces 3's.

Critical Observation

To remove `cnt3` threes, we need **exactly** `cnt3` divisions by 6.

Each division also removes one 2.

So after removing all 3's:

$$\text{Remaining 2's} = cnt2 - cnt3$$

To be valid, after all operations we must reach exponent of 2 equal to 0.

Thus:

$$cnt2 - cnt3 \leq 0$$

→ If:

× $cnt2 > cnt3 \rightarrow \text{impossible}$

Because divide-by-6 removes 2's and 3's equally.

You don't have enough 3's to "pair" with extra 2's.

✓ STEP 4 — If valid: compute moves

We need:

- exactly `cnt3` divide-by-6 operations (to kill 3's)
- if $cnt2 < cnt3$, we must **multiply by 2** to increase exponent of 2 until they match

Each multiply-by-2 increases exponent of 2 by 1.

We need:

$$(cnt3 - cnt2) \text{ multiplications}$$

Total moves:

$$(cnt3 - cnt2) + cnt3 = 2 \cdot cnt3 - cnt2$$

This matches code:

```
2 * cnt3 - cnt2
```

 Copy code

✓ FINAL FORMULA (Proven)

If n contains primes other than 2 or 3 $\rightarrow -1$

Else:

- If $\text{cnt2} > \text{cnt3} \rightarrow -1$
- Else:

$$\text{answer} = (\text{cnt3} - \text{cnt2}) + \text{cnt3} = 2\text{cnt3} - \text{cnt2}$$

🔥 Example Proof Works

Example: $n = 12 = 2^2 * 3^1$

$\text{cnt2} = 2, \text{cnt3} = 1$

Check: $\text{cnt2} > \text{cnt3}$

\rightarrow impossible

Output: -1

Matches sample.

Example: $n = 36 = 2^2 * 3^2$

$\text{cnt2} = 2, \text{cnt3} = 2$

valid

Moves:

- need $\text{cnt3} = 2$ divides
- need $\text{cnt3} - \text{cnt2} = 0$ multiplies

Total = $2*2 - 2 = 2$

Matches.

🎉 Final Result

This proves the CF editorial logic:

✓ If other primes → return `-1`

✓ If `cnt2 > cnt3` → return `-1`

✓ Else return `2 * cnt3 - cnt2`

If you want, I can also give you a **step-by-step intuitive explanation**, a **diagram proof**, or help you **implement your own solution**.

